Add a PwAffList abstract domain.

PFunc.v
@@ -1,11 +1,12 @@
 From Coq Require Import ssreflect ssrfun ssrbool.
-From Coq Require Export Arith.Arith Strings.String.
+From Coq Require Export Strings.String ZArith.BinInt.
+Local Open Scope Z_scope.
+
 Local Set Warnings "-notation-overridden".
-From mathcomp Require Import ssreflect.ssrnat.
 
 Inductive V :=
 | VTop
-| VVal (n: nat)
+| VVal (n: Z)
 | VBot.
 
 Definition le_V (v1 v2: V) :=
@@ -13,8 +14,61 @@ Definition le_V (v1 v2: V) :=
   | (_, VTop) => true
   | (VBot, _) => true
   | (VVal n1, VVal n2) => n1 =? n2
-  | _ => false
+  |
+  _ => false
   end.
+
+Theorem le_V_refl : forall v, (le_V v v).
+Proof.
+  case => // n.
+  rewrite /le_V.
+  by apply Z.eqb_refl.
+Qed.
+
+Theorem le_V_trans :
+  forall v1 v2 v3, le_V v1 v2 -> le_V v2 v3 -> le_V v1 v3.
+Proof.
+  move => v1 v2 v3.
+  case v1; case v2; case v3 => //.
+  rewrite /le_V.
+  move => n3 n2 n1 /Z.eqb_spec H12 /Z.eqb_spec H23.
+  rewrite H12 H23.
+    by apply /Z.eqb_spec.
+Qed.
+
+Definition in_V (n: Z) (v: V) :=
+  match v with
+  | VTop => true
+  | VVal n' => n =? n'
+  | VBot => false
+  end.
+
+Definition le_V_spec :
+  forall v1 v2, le_V v1 v2 <-> forall n, in_V n v1 -> in_V n v2.
+Proof.
+  move => v1 v2.
+  split.
+  - case v1; case v2 => // n n0.
+    rewrite /le_V => /Z.eqb_spec -> //.
+  - case v1; case v2 => //.
+    + move => n /= Hin.
+      move: (Hin (n+1) is_true_true) => Himpossible.
+        by rewrite /is_true Z.add_1_r Z.eqb_compare Zcompare.Zcompare_succ_Gt in Himpossible.
+    + move => Hle.
+        by have /Hle : (in_V 0 VTop) by [] => Himpossible.
+    + move => n n0 Hin.
+      case (Z.eqb_spec n n0).
+      * move => Heq.
+          by rewrite Heq /le_V Z.eqb_refl.
+      * move => /Z.eqb_spec Hne.
+        move: (Hin n0) => Himpossible.
+        have /Himpossible : (in_V n0 (VVal n0)). by rewrite /in_V Z.eqb_refl.
+          by rewrite /in_V.
+    + move => n Hin.
+      move: (Hin n) => Hin'.
+      have /Hin' : (in_V n (VVal n)). by rewrite /in_V Z.eqb_refl.
+        by move => Himpossible.
+Qed.
 
 Class PFuncImpl (PFunc: Type) :=
   {
@@ -30,3 +84,26 @@ Class PFuncImpl (PFunc: Type) :=
     join_pfunc_spec_l : forall p1 p2, le_pfunc p1 (join_pfunc p1 p2);
     join_pfunc_spec_r : forall p1 p2, le_pfunc p2 (join_pfunc p1 p2);
   }.
+
+Theorem le_pfunc_refl {PFunc: Type} {PI: PFuncImpl PFunc} :
+  forall a, le_pfunc a a.
+Proof.
+  move => a.
+  apply le_pfunc_spec => x.
+  apply le_V_refl.
+Qed.
+
+Theorem le_pfunc_trans {PFunc: Type} {PI: PFuncImpl PFunc} :
+  forall a1 a2 a3, le_pfunc a1 a2 -> le_pfunc a2 a3 -> le_pfunc a1 a3.
+Proof.
+  move => a1 a2 a3 /le_pfunc_spec H12 /le_pfunc_spec H23.
+  apply le_pfunc_spec => x.
+    by apply (le_V_trans _ (eval_pfunc a2 x)).
+Qed.
+
+Ltac simpl_pfunc :=
+  repeat (
+      rewrite ?le_V_refl ?constant_pfunc_spec ?join_pfunc_spec_l ?join_pfunc_spec_r
+              ?le_pfunc_refl
+    ).
+
